src/HOL/SMT_Examples/SMT_Word_Examples.thy
@@ -11,7 +11,7 @@ begin
 declare [[smt_oracle = true]]
 declare [[z3_extensions = true]]
 declare [[smt_certificates = "SMT_Word_Examples.certs"]]
-declare [[smt_read_only_certificates = true]]
+declare [[smt_read_only_certificates = false]]
 
 text \<open>
 Currently, there is no proof reconstruction for words.
